SystemMp.lean
@@ -1,3 +1,5 @@
 -- This module serves as the root of the `SystemMp` library.
 -- Import modules here that should be built as part of the library.
 import «SystemMp».Basic
+import «SystemMp».Definitions
+import «SystemMp».Infrastructure
