SystemMp/Assoc.lean
@@ -1,0 +1,16 @@
+import SystemMp.Basic
+import Aesop
+
+namespace SystemMP
+
+open SystemMP
+
+namespace Assoc
+
+def Pair.{u} {α : Type u} := (Atom × α)
+
+def dom(Γ : List (@Pair α)) : List Atom := Γ.map Prod.fst
+
+instance [BEq α] : BEq (@Pair α) where
+  beq x y := x.1 == y.1 && x.2 == y.2
+
