SystemMp/Infrastructure.lean
@@ -1,0 +1,26 @@
+import «SystemMp».Definitions
+import Aesop
+
+open SystemMP
+open binding
+
+theorem env_binds_equal_var {Γ : Env} {x : Atom} {U T : Typ} :
+    Wf_Env Γ →
+    Γ.contains (x, bind_val U) →
+    Γ.contains (x, bind_val T) →
+    U = T := by 
+      intro wf bu bt
+      match wf with
+      | .W_nil => cases bu
+      | .W_val Γ2 x' T' x'notinΓ2 T'wf =>
+        sorry
+        -- cases bu
+        -- · cases bt
+        --   · rfl
+        --   · sorry
+        -- · cases bt
+        --   · sorry
+        --   · sorry
+      | .W_typ Γ2 X T' XnotinΓ2 T'wf =>
+        sorry
+
