lakefile.lean
@@ -11,6 +11,9 @@ package «system-mp» where
 require mathlib from git
   "https://github.com/leanprover-community/mathlib4.git"
 
+require aesop from git 
+  "https://github.com/leanprover-community/aesop"
+
 @[default_target]
 lean_lib «SystemMp» where
   -- add any library configuration options here
